src/HaskStrongTypes.v
@@ -4,11 +4,82 @@
 
 Generalizable All Variables.
 Require Import Preamble.
-Require Import General.
 Require Import Coq.Strings.String.
 Require Import Coq.Lists.List.
-Require Import HaskGeneral.
-Require Import HaskLiterals.
+Require Import General.
+Require Import HaskKinds.
+Require Import HaskCoreLiterals.
+Require Import HaskCoreTypes.  (* FIXME *)
+Require Import HaskCoreVars.   (* FIXME *)
+Require Import HaskWeakTypes.
+Require Import HaskWeakVars.   (* FIXME *)
+Require Import HaskCoreToWeak. (* FIXME *)
+
+Variable CoFunConst        : nat -> Type.  (* FIXME *)
+Variable TyFunConst        : nat -> Type.  (* FIXME *)
+
+Variable dataConTyCon      : CoreDataCon -> TyCon.     Extract Inlined Constant dataConTyCon => "DataCon.dataConTyCon".
+
+Variable dataConExVars_    : CoreDataCon -> list CoreVar.  Extract Inlined Constant dataConExVars_ => "DataCon.dataConExTyVars".
+Variable dataConEqTheta_   : CoreDataCon -> list PredType. Extract Inlined Constant dataConEqTheta_ => "DataCon.dataConEqTheta".
+Variable dataConOrigArgTys_:CoreDataCon -> list CoreType. Extract Inlined Constant dataConOrigArgTys_ =>"DataCon.dataConOrigArgTys".
+Variable getTyConTyVars_   : TyCon   -> list CoreVar.  Extract Inlined Constant getTyConTyVars_ => "TyCon.tyConTyVars".
+
+(* FIXME: might be a better idea to panic here than simply drop things that look wrong *)
+Definition tyConTyVars (tc:TyCon) :=
+  filter (map (fun x => match coreVarToWeakVar x with WTypeVar v => Some v | _ => None end) (getTyConTyVars_ tc)).
+  Opaque tyConTyVars.
+Definition dataConExTyVars cdc :=
+  filter (map (fun x => match coreVarToWeakVar x with WTypeVar v => Some v | _ => None end) (dataConExVars_ cdc)).
+  Opaque dataConExTyVars.
+Definition dataConCoerKinds cdc :=
+  filter (map (fun x => match x with EqPred t1 t2 =>
+                          match (
+                            coreTypeToWeakType t1 >>= fun t1' =>
+                              coreTypeToWeakType t2 >>= fun t2' =>
+                                OK (t1',t2'))
+                          with OK z => Some z
+                            | _ => None
+                          end
+                          | _ => None
+                        end) (dataConEqTheta_ cdc)).
+  Opaque dataConCoerKinds.
+Definition dataConFieldTypes cdc :=
+  filter (map (fun x => match coreTypeToWeakType x with
+                          | OK z => Some z
+                          | _ => None
+                        end) (dataConOrigArgTys_ cdc)).
+
+Definition tyConNumKinds (tc:TyCon) := length (tyConTyVars tc).
+  Coercion tyConNumKinds : TyCon >-> nat.
+
+Inductive DataCon : TyCon -> Type :=
+  mkDataCon : forall cdc:CoreDataCon, DataCon (dataConTyCon cdc).
+  Definition dataConToCoreDataCon `(dc:DataCon tc) : CoreDataCon := match dc with mkDataCon cdc => cdc end.
+  Coercion mkDataCon : CoreDataCon >-> DataCon.
+  Coercion dataConToCoreDataCon : DataCon >-> CoreDataCon.
+  (*Opaque DataCon.*)
+
+Definition compare_datacons : forall tc, forall dc1 dc2:DataCon tc, bool.
+  intros.
+  destruct dc1.
+  destruct dc2.
+  exact (if eqd_dec cdc cdc0 then true else false).
+  Defined.
+
+Axiom trust_compare_datacons : forall tc dc1 dc2, if compare_datacons tc dc1 dc2 then dc1=dc2 else not (dc1=dc2).
+
+Instance DataConEqDecidable : forall tc, EqDecidable (@DataCon tc).
+  intros.
+  apply Build_EqDecidable.
+  intros.
+  set (trust_compare_datacons _ v1 v2) as x.
+  set (compare_datacons tc v1 v2) as y.
+  assert (y=compare_datacons tc v1 v2). reflexivity.
+  destruct y; rewrite <- H in x.
+  left; auto.
+  right; auto.
+  Defined.
 
 (* types prefixed with "Raw" are NOT binder-polymorphic; they have had their PHOAS parameter instantiated already *)
 Section Raw.
@@ -19,13 +90,14 @@ Section Raw.
   (* Figure 7: ρ, σ, τ, ν *)
   Inductive RawHaskType  : Type :=
   | TVar           : TV                                                     -> RawHaskType   (* a        *)
-  | TCon           : ∀n, TyCon n                                            -> RawHaskType   (* T        *)
-  | TCoerc         : Kind                                                   -> RawHaskType   (* (+>)     *)
+  | TCon           : TyCon                                                  -> RawHaskType   (* T        *)
+  | TArrow         :                                                           RawHaskType   (* (->)     *)
+  | TCoerc         : RawHaskType -> RawHaskType -> RawHaskType              -> RawHaskType   (* (+>)     *)
   | TApp           : RawHaskType                  ->     RawHaskType        -> RawHaskType   (* φ φ      *)
-  | TFCApp         : ∀n, TyFunConst n             -> vec RawHaskType n      -> RawHaskType   (* S_n      *)
+  | TFCApp         : forall tc:TyCon,                vec RawHaskType tc     -> RawHaskType   (* S_n      *)
   | TAll           : Kind  -> (TV -> RawHaskType)                           -> RawHaskType   (* ∀a:κ.φ   *)
   | TCode          : RawHaskType -> RawHaskType                             -> RawHaskType   (* from λ^α *).
-
+    
   (* the "kind" of a coercion is a pair of types *)
   Inductive RawCoercionKind : Type := mkRawCoercionKind : RawHaskType -> RawHaskType -> RawCoercionKind.
 
@@ -40,8 +112,8 @@ Section Raw.
     | CoType         : RawHaskType                                  -> RawHaskCoer (* τ      *)
     | CoApp          : RawHaskCoer -> RawHaskCoer                   -> RawHaskCoer (* γ γ    *)
     | CoAppT         : RawHaskCoer -> RawHaskType                   -> RawHaskCoer (* γ@v    *)
-    | CoCFApp        : ∀n, CoFunConst n -> vec RawHaskCoer n        -> RawHaskCoer (* C   γⁿ *)
-    | CoTFApp        : ∀n, TyFunConst n -> vec RawHaskCoer n        -> RawHaskCoer (* S_n γⁿ *)
+    | CoCFApp        : ∀ n, CoFunConst n -> vec RawHaskCoer n       -> RawHaskCoer (* C   γⁿ *)
+    | CoTFApp        : ∀ n, TyFunConst n -> vec RawHaskCoer n       -> RawHaskCoer (* S_n γⁿ *)
     | CoAll          : Kind  -> (TV -> RawHaskCoer)                 -> RawHaskCoer (* ∀a:κ.γ *)
     | CoSym          : RawHaskCoer                                  -> RawHaskCoer (* sym    *)
     | CoComp         : RawHaskCoer -> RawHaskCoer                   -> RawHaskCoer (* ◯      *)
@@ -51,15 +123,14 @@ Section Raw.
   End CV.
 End Raw.
 
-Implicit Arguments TCon   [ [TV] [n]].
-Implicit Arguments TFCApp [ [TV] [n]].
+Implicit Arguments TCon   [ [TV] ].
+Implicit Arguments TFCApp [ [TV] ].
 Implicit Arguments RawHaskType  [ ].
 Implicit Arguments RawHaskCoer  [ ].
 Implicit Arguments RawCoercionKind [ ].
 
-Notation "t1 ---> t2"        := (fun TV env => (@TApp _ (@TApp _ (@TCon TV _ ArrowTyCon) (t1 TV env)) (t2 TV env))).
-Notation "φ₁ ∼∼ φ₂ : κ ⇒ φ₃" :=
-   (fun TV env => @TApp _ (@TApp _ (@TCon _ _ ArrowTyCon) (@TApp _ (@TApp _ (@TCoerc _ κ) (φ₁ TV env)) (φ₂ TV env))) (φ₃ TV env)).
+Notation "t1 ---> t2"        := (fun TV env => (TApp (TApp TArrow (t1 TV env)) (t2 TV env))).
+Notation "φ₁ ∼∼ φ₂ ⇒ φ₃"     := (fun TV env => TCoerc (φ₁ TV env) (φ₂ TV env) (φ₃ TV env)).
 
 
 
@@ -94,10 +165,13 @@ Definition HaskTAll {Γ}(κ:Kind)(σ:forall TV (env:@InstantiatedTypeEnv TV Γ),
 Definition HaskTApp {Γ}(σ:forall TV (env:@InstantiatedTypeEnv TV Γ), TV -> RawHaskType TV)(cv:HaskTyVar Γ) : HaskType Γ
   := fun TV env => σ TV env (cv TV env).
 Definition HaskBrak {Γ}(v:HaskTyVar Γ)(t:HaskType Γ) : HaskType Γ := fun TV env => @TCode TV (TVar (v TV env)) (t TV env).
-Definition HaskTCon {Γ}{n}(tc:TyCon n) : HaskType Γ := fun TV ite => TCon tc.
+Definition HaskTCon {Γ}(tc:TyCon) : HaskType Γ := fun TV ite => TCon tc.
 Definition HaskAppT {Γ}(t1 t2:HaskType Γ) : HaskType Γ := fun TV ite => TApp (t1 TV ite) (t2 TV ite).
 Definition mkHaskCoercionKind {Γ}(t1 t2:HaskType Γ) : HaskCoercionKind Γ :=
  fun TV ite => mkRawCoercionKind (t1 TV ite) (t2 TV ite).
+Definition unMkHaskCoercionKind {Γ}(hck:HaskCoercionKind Γ) : (HaskType Γ * HaskType Γ) :=
+  ((fun TV ite => match (hck TV ite) with mkRawCoercionKind t1 _ => t1 end),
+   (fun TV ite => match (hck TV ite) with mkRawCoercionKind _ t2 => t2 end)).
 
 
 (* PHOAS substitution on types *)
@@ -108,15 +182,16 @@ Definition substT {Γ}(exp:forall TV (env:@InstantiatedTypeEnv TV Γ), TV -> Raw
     | TVar       x        => x
     | TAll       k y      => TAll      k (fun v => flattenT (y (TVar v)))
     | TApp       x y      => TApp      (flattenT x) (flattenT y)
-    | TCon   n   tc       => TCon      tc
-    | TCoerc     k        => TCoerc    k
+    | TCon       tc       => TCon      tc
+    | TCoerc t1 t2   t    => TCoerc    (flattenT t1) (flattenT t2)   (flattenT t)
+    | TArrow              => TArrow
     | TCode      v e      => TCode     (flattenT v) (flattenT e)
-    | TFCApp     n tfc lt => TFCApp    tfc
+    | TFCApp       tfc lt => TFCApp    tfc
       ((fix flatten_vec n (expv:vec (RawHaskType (RawHaskType TV)) n) : vec (RawHaskType TV) n :=
         match expv in vec _ N return vec (RawHaskType TV) N with
           | vec_nil => vec_nil
           | x:::y   => (flattenT x):::(flatten_vec _ y)
-        end) n lt)
+        end) _ lt)
     end)
     (exp (RawHaskType TV) (vec_map (fun tv => TVar tv) env) (v TV env)).
 Notation "t @@  l" := (@mkLeveledHaskType _ t l) (at level 20).
@@ -125,21 +200,6 @@ Notation "'<[' a '|-' t ']>'" := (@HaskBrak _ a t).
 
 
 
-(* like a GHC DataCon, but using PHOAS representation for types and coercions *)
-Record StrongAltConInfo {n}{tc:TyCon n} :=
-{ saci_numExTyVars :  nat
-; saci_numCoerVars :  nat
-; saci_numExprVars :  nat
-; saci_akinds      :  vec Kind n
-; saci_ekinds      :  vec Kind saci_numExTyVars
-; saci_kinds       := app (vec2list saci_akinds) (vec2list saci_ekinds)
-; saci_coercions   :  vec (HaskType saci_kinds * HaskType saci_kinds) saci_numCoerVars
-; saci_types       :  vec (HaskType saci_kinds) saci_numExprVars
-}.
-Implicit Arguments StrongAltConInfo [[n]].
-
-Definition caseType {Γ:TypeEnv}{n}(tc:TyCon n)(atypes:vec (HaskType Γ) n) :=
-  fold_left HaskAppT (vec2list atypes) (HaskTCon(Γ:=Γ) tc).
 
 
 
@@ -151,7 +211,7 @@ Definition caseType {Γ:TypeEnv}{n}(tc:TyCon n)(atypes:vec (HaskType Γ) n) :=
 
 
 
-(* FIXME: it's a mess below this point *)
+(* yeah, things are kind of messy below this point *)
 
 
 Definition unAddKindFromInstantiatedTypeEnv {Γ:TypeEnv}{κ:Kind}{TV:Type}(ite:InstantiatedTypeEnv TV (κ::Γ)) := vec_tail ite.
@@ -209,6 +269,15 @@ Definition lamer {a}{b}{c}(lt:HaskType (app (app a  b) c)) : HaskType  (app a (a
 rewrite <- ass_app in lt.
 exact lt.
 Defined.
+Definition weakCK {Γ}{κ}(hck:HaskCoercionKind Γ) : HaskCoercionKind (κ::Γ) :=
+  let (t1,t2) := unMkHaskCoercionKind hck in mkHaskCoercionKind (weakT t1) (weakT t2).
+Definition weakCK' {Γ}{κ}(hck:HaskCoercionKind Γ) : HaskCoercionKind (app κ Γ) :=
+  let (t1,t2) := unMkHaskCoercionKind hck in mkHaskCoercionKind (weakT' t1) (weakT' t2).
+Definition weakCK'' {Γ}{κ}(hck:list (HaskCoercionKind Γ)) : list (HaskCoercionKind (app κ Γ)) :=
+match κ as K return list (HaskCoercionKind (app K Γ)) with
+  | nil => hck
+  | _   => map weakCK' hck
+end.
 Definition weakL' {Γ}{κ}(lev:HaskLevel Γ) : HaskLevel (app κ Γ).
   induction κ; auto. apply weakL; auto. Defined.
 Definition weakLT {Γ}{κ}(lt:LeveledHaskType Γ) : LeveledHaskType (κ::Γ) := match lt with t @@ l => weakT t @@ weakL l end.
@@ -237,11 +306,31 @@ Definition weakF {Γ:TypeEnv}{κ:Kind}(f:forall TV (env:@InstantiatedTypeEnv TV 
   forall TV (env:@InstantiatedTypeEnv TV (κ::Γ)), TV -> RawHaskType TV
   := fun TV ite tv => (f TV (weakITE ite) tv).
 
+(* like a GHC DataCon, but using PHOAS representation for types and coercions *)
+Record StrongAltCon {tc:TyCon} :=
+{ sac_altcon      :  AltCon
+; sac_numExTyVars :  nat
+; sac_numCoerVars :  nat
+; sac_numExprVars :  nat
+; sac_akinds      :  vec Kind tc
+; sac_ekinds      :  vec Kind sac_numExTyVars
+; sac_kinds       := app (vec2list sac_akinds) (vec2list sac_ekinds)
+; sac_Γ           := fun Γ => app (vec2list sac_ekinds) Γ
+; sac_coercions   :  forall Γ (atypes:vec (HaskType Γ) tc), vec (HaskCoercionKind (sac_Γ Γ)) sac_numCoerVars
+; sac_types       :  forall Γ (atypes:vec (HaskType Γ) tc), vec (HaskType (sac_Γ Γ)) sac_numExprVars
+; sac_Δ           := fun    Γ (atypes:vec (HaskType Γ) tc) Δ => app (vec2list (sac_coercions Γ atypes)) Δ
+}.
+Coercion sac_altcon : StrongAltCon >-> AltCon.
+
+Definition caseType {Γ:TypeEnv}(tc:TyCon)(atypes:vec (HaskType Γ) tc) :=
+  fold_left HaskAppT (vec2list atypes) (HaskTCon(Γ:=Γ) tc).
+
+
 (***************************************************************************************************)
 (* Well-Formedness of Types and Coercions                                                          *)
 (* also represents production "S_n:κ" of Γ because these can only wind up in Γ via rule (Type) *)
-Inductive TypeFunctionDecl (n:nat)(tfc:TyFunConst n)(vk:vec Kind n) : Type :=
-  mkTFD : Kind -> TypeFunctionDecl n tfc vk.
+Inductive TypeFunctionDecl (tfc:TyCon)(vk:vec Kind tfc) : Type :=
+  mkTFD : Kind -> TypeFunctionDecl tfc vk.
 
 
 (* Figure 8, upper half *)
@@ -257,8 +346,8 @@ Inductive WellKinded_RawHaskType (TV:Type)
   | WFTyAll  : forall Γ (env:InstantiatedTypeEnv TV Γ) κ     σ    ,
                 (∀ a, WellKinded_RawHaskType TV _ (@addKindToInstantiatedTypeEnv _ TV env a κ) (σ a) ★ )        -> 
                 WellKinded_RawHaskType TV _  env      (TAll κ σ) ★ 
-  | TySCon   : forall Γ env n tfc lt vk ι ,
-                @TypeFunctionDecl n tfc vk  ->
+  | TySCon   : forall Γ env tfc lt vk ι ,
+                @TypeFunctionDecl tfc vk  ->
                 ListWellKinded_RawHaskType TV Γ _ env lt vk ->
                 WellKinded_RawHaskType TV Γ env (TFCApp tfc lt) ι
 with ListWellKinded_RawHaskType (TV:Type)
@@ -270,31 +359,41 @@ with ListWellKinded_RawHaskType (TV:Type)
                 ListWellKinded_RawHaskType TV Γ n env     lt      lk  ->
                 ListWellKinded_RawHaskType TV Γ (S n) env  (t:::lt) (k:::lk).
 
-(*
-Fixpoint kindOfRawHaskType {TV}(rht:RawHaskType Kind) : Kind :=
+Variable kindOfTyCon : forall (tc:TyCon), Kind.
+  Extract Inlined Constant kindOfTyCon => "(\x -> Prelude.error ""not implemented yet"")".
+
+Fixpoint kindOfRawHaskType (rht:RawHaskType Kind) : ???Kind :=
 match rht with
-  | TVar   k    => k
-  | TCon   n tc => ̱★ (* FIXME: use the StrongAltConInfo *)
-  | TCoerc k    => k ⇛ (k ⇛ (★ ⇛ ★ ))
-  | TApp   ht1 ht2        : RawHaskType                  ->     RawHaskType        -> RawHaskType   (* φ φ      *)
-  | TFCApp         : ∀n, TyFunConst n             -> vec RawHaskType n      -> RawHaskType   (* S_n      *)
-  | TAll           : Kind  -> (TV -> RawHaskType)                           -> RawHaskType   (* ∀a:κ.φ   *)
-  | TCode          : RawHaskType -> RawHaskType                             -> RawHaskType   (* from λ^α *).
-*)
+  | TVar   k         => OK k
+  | TCon     tc      => OK (kindOfTyCon tc)
+  | TCoerc t1 t2   t => OK (★ ⇛ ★ )
+  | TArrow           => OK (★ ⇛ ★ ⇛ ★ )
+  | TApp   ht1 ht2   => kindOfRawHaskType ht1 >>= fun k1 =>
+                        kindOfRawHaskType ht2 >>= fun k2 =>
+                          match k1 with
+                            | k1' ⇛ k2' => if eqd_dec k1' k1 then OK k2' else Error "kind mismatch"
+                            | _         =>                                    Error "attempt to apply a non-functional kind"
+                          end
+  | TFCApp   tc rht' => Error "calculating kind of TFCApp is not yet implemented"
+  | TAll   k t'      => kindOfRawHaskType (t' k) >>= fun k' => OK (k ⇛ k')
+  | TCode  t1 t2     => OK ★
+end.
+
+Definition kindITE (Γ:TypeEnv) : InstantiatedTypeEnv Kind Γ :=
+  list2vec Γ.
+
+Definition kindOfType {Γ}(ht:HaskType Γ) : ???Kind :=
+  kindOfRawHaskType (ht Kind (kindITE Γ)).
+
 Definition WellKindedHaskType Γ (ht:HaskType Γ) κ :=
   forall TV env, WellKinded_RawHaskType TV Γ env (ht TV env) κ.
   Notation "Γ '⊢ᴛy' σ : κ" := (WellKindedHaskType Γ σ κ).
-
-
 
 (* "decl", production for "axiom" *)
 Structure AxiomDecl (n:nat)(ccon:CoFunConst n)(vk:vec Kind n){TV:Type} : Type :=
 { axd_τ : vec TV n -> RawHaskType TV
 ; axd_σ : vec TV n -> RawHaskType TV
 }.
-
-
-
 
 Section WFCo.
   Context {TV:Type}.
@@ -311,8 +410,7 @@ Section WFCo.
   Inductive WFCoercion:forall Γ (Δ:CoercionEnv Γ),
     @InstantiatedTypeEnv TV Γ ->
     @InstantiatedCoercionEnv TV CV Γ Δ ->
-    @RawHaskCoer TV CV -> @RawCoercionKind TV -> Prop :=.
-(*
+    @RawHaskCoer TV CV -> @RawCoercionKind TV -> Prop :=
   | CoTVar':∀ Γ Δ t e c σ τ,
     (@coercionEnvContainsCoercion Γ _ TV CV t e c (@mkRawCoercionKind _ σ τ)) -> e⊢ᴄᴏ CoVar c : σ ∼ τ  : Δ : Γ : t
   | CoRefl :∀ Γ Δ t e   τ κ,                                         t ⊢ᴛy τ :κ    -> e⊢ᴄᴏ CoType τ    :         τ ∼ τ  : Δ :Γ: t
@@ -320,6 +418,7 @@ Section WFCo.
   | Trans  :∀ Γ Δ t e γ₁ γ₂ σ₁ σ₂ σ₃,(e⊢ᴄᴏ γ₁:σ₁∼σ₂:Δ:Γ:t) -> (e⊢ᴄᴏ γ₂:σ₂∼σ₃:Δ:Γ:t) -> e⊢ᴄᴏ CoComp γ₁ γ₂:        σ₁ ∼ σ₃ : Δ :Γ: t
   | Left   :∀ Γ Δ t e γ σ₁ σ₂ τ₁ τ₂,(e⊢ᴄᴏ γ : TApp σ₁ σ₂ ∼ TApp τ₁ τ₂ :Δ:Γ:t    )  -> e⊢ᴄᴏ CoLeft  γ   :        σ₁ ∼ τ₁ : Δ :Γ: t
   | Right  :∀ Γ Δ t e γ σ₁ σ₂ τ₁ τ₂,(e⊢ᴄᴏ γ : TApp σ₁ σ₂ ∼ TApp τ₁ τ₂ :Δ:Γ:t   )   -> e⊢ᴄᴏ CoRight γ   :        σ₂ ∼ τ₂ : Δ :Γ: t
+  (*
   | SComp  :∀ Γ Δ t e γ n S σ τ κ,
             ListWFCo Γ Δ t e γ σ τ -> t ⊢ᴛy TFCApp(n:=n) S σ : κ  -> e⊢ᴄᴏ CoTFApp S γ : TFCApp S σ∼TFCApp S τ : Δ : Γ : t
   | CoAx   :∀ Γ Δ t e n C κ γ, forall (σ₁:vec TV n) (σ₂:vec TV n), forall (ax:@AxiomDecl n C κ TV),
@@ -327,17 +426,15 @@ Section WFCo.
     ListWellKinded_RawHaskType TV Γ t   (map TVar (vec2list σ₁))            (vec2list κ)  ->
     ListWellKinded_RawHaskType TV Γ t   (map TVar (vec2list σ₂))            (vec2list κ)  ->
     e⊢ᴄᴏ CoCFApp C γ : axd_σ _ _ _ ax σ₁ ∼ axd_τ _ _ _ ax σ₂ : Δ : Γ : t
-
+  *)
   | WFCoAll  : forall Γ Δ κ (t:InstantiatedTypeEnv TV Γ) (e:InstantiatedCoercionEnv TV CV (κ::Γ) (weakCE Δ)) γ σ τ    ,
       (∀ a,           e ⊢ᴄᴏ (        γ a) : (       σ a) ∼ (       τ a) : _ : _ : (t + a : κ))
       ->    weakICE e ⊢ᴄᴏ (CoAll κ γ  ) : (TAll κ σ  ) ∼ (TAll κ τ  ) : Δ : Γ :  t
-
   | Comp   :forall Γ Δ t e γ₁ γ₂ σ₁ σ₂ τ₁ τ₂ κ,
             (t ⊢ᴛy TApp σ₁ σ₂:κ)->
             (e⊢ᴄᴏ γ₁:σ₁∼τ₁:Δ:Γ:t)->
             (e⊢ᴄᴏ γ₂:σ₂∼τ₂:Δ:Γ:t) ->
             e⊢ᴄᴏ (CoApp γ₁ γ₂) : (TApp σ₁ σ₂) ∼ (TApp τ₁ τ₂) : Δ:Γ:t
-
   | CoInst :forall Γ Δ t e σ τ κ γ (v:∀ TV, InstantiatedTypeEnv TV Γ -> RawHaskType TV),
           t ⊢ᴛy v TV t : κ  ->
             (e⊢ᴄᴏ γ:HaskTAll κ σ _ t ∼ HaskTAll κ τ _ t:Δ:Γ:t) ->
@@ -350,7 +447,6 @@ Section WFCo.
   | LWFCo_cons : ∀ Γ Δ t e a b c la lb lc, (e⊢ᴄᴏ a : b∼c : Δ : Γ : t )->
     ListWFCo Γ Δ t e la lb lc -> ListWFCo Γ Δ t e (a::la) (b::lb) (c::lc)
   where "ice '⊢ᴄᴏ' γ : a '∼' b : Δ : Γ : ite" := (@WFCoercion Γ Δ ite ice γ (@mkRawCoercionKind _ a b)).
-*)
 End WFCo.
 
 Definition WFCCo (Γ:TypeEnv)(Δ:CoercionEnv Γ)(γ:HaskCoercion Γ Δ)(a b:HaskType Γ) :=
@@ -358,9 +454,9 @@ Definition WFCCo (Γ:TypeEnv)(Δ:CoercionEnv Γ)(γ:HaskCoercion Γ Δ)(a b:Hask
     @WFCoercion _ _ Γ Δ env cenv (γ TV CV env cenv) (@mkRawCoercionKind _ (a TV env) (b TV env)).
     Notation "Δ '⊢ᴄᴏ' γ : a '∼' b" := (@WFCCo _ Δ γ a b).
 
-  Definition literalType (lit:HaskLiteral){Γ} : HaskType Γ := fun TV ite => (TCon (haskLiteralToTyCon lit)).
-  Notation "a ∼∼∼ b" := (mkHaskCoercionKind a b) (at level 18).
+Definition literalType (lit:HaskLiteral){Γ} : HaskType Γ := fun TV ite => (TCon (haskLiteralToTyCon lit)).
 
+Notation "a ∼∼∼ b" := (mkHaskCoercionKind a b) (at level 18).
 
 Fixpoint update_ξ
   `{EQD_VV:EqDecidable VV}{Γ}(ξ:VV -> LeveledHaskType Γ)(vt:list (VV * LeveledHaskType Γ)) : VV -> LeveledHaskType Γ :=
@@ -368,29 +464,3 @@ Fixpoint update_ξ
     | nil => ξ
     | (v,τ)::tl => fun v' => if eqd_dec v v' then τ else (update_ξ ξ tl) v'
   end.
-
-
-
-
-
-
-
-
-
-
-
-
-
-
-
-
-(* just like GHC's AltCon, but using PHOAS types and coercions *)
-Record StrongCaseBranch {n}{tc:TyCon n}{Γ}{atypes:vec (HaskType Γ) n} :=
-{ scb_saci      :  @StrongAltConInfo _ tc
-; scb_Γ         :  TypeEnv := app (vec2list (saci_ekinds scb_saci)) Γ
-; scb_Δ         :  CoercionEnv scb_Γ
-; scb_types     :  vec (LeveledHaskType (app (vec2list (saci_ekinds scb_saci)) Γ)) (saci_numExprVars scb_saci)
-}.
-Coercion scb_saci : StrongCaseBranch >-> StrongAltConInfo.
-Implicit Arguments StrongCaseBranch [[n][Γ]].
-
