src/HaskKinds.v
@@ -1,0 +1,38 @@
+(*********************************************************************************************************************************)
+(* HaskKinds:  Definitions shared by all four representations (Core, Weak, Strong, Proof)                                      *)
+(*********************************************************************************************************************************)
+
+Generalizable All Variables.
+Require Import Preamble.
+Require Import General.
+Require Import Coq.Strings.String.
+Open Scope nat_scope.
+
+Variable Note                : Type.                         Extract Inlined Constant Note       => "CoreSyn.Note".
+Variable nat2string          : nat         -> string.        Extract Inlined Constant nat2string            => "nat2string".
+
+(* Figure 7: production κ, ι *)
+Inductive Kind : Type := 
+  | KindType         : Kind                      (* ★  - the kind of boxed types*)
+  | KindTypeFunction : Kind  -> Kind  -> Kind    (* ⇛ *)
+  | KindUnliftedType : Kind                      (* not in the paper - this is the kind of unboxed non-tuple types *)
+  | KindUnboxedTuple : Kind                      (* not in the paper - this is the kind of unboxed tuples *)
+  | KindArgType      : Kind                      (* not in the paper - this is the lub of KindType and KindUnliftedType *)
+  | KindOpenType     : Kind                      (* not in the paper - kind of all types (lifted, boxed, whatever) *).
+
+Notation "'★'"   := KindType.
+Notation "a ⇛ b" := (KindTypeFunction a b).
+
+Instance KindEqDecidable : EqDecidable Kind.
+  apply Build_EqDecidable.
+  induction v1.
+    destruct v2; try (right; intro q; inversion q; fail) ; left ; auto.
+    destruct v2; try (right; intro q; inversion q; fail) ; auto.
+      destruct (IHv1_1 v2_1); destruct (IHv1_2 v2_2); subst; auto;
+      right; intro; subst; inversion H; subst; apply n; auto.
+    destruct v2; try (right; intro q; inversion q; fail) ; left ; auto.
+    destruct v2; try (right; intro q; inversion q; fail) ; left ; auto.
+    destruct v2; try (right; intro q; inversion q; fail) ; left ; auto.
+    destruct v2; try (right; intro q; inversion q; fail) ; left ; auto.
+  Defined.
+
