src/HaskWeakTypes.v
@@ -1,0 +1,132 @@
+(*********************************************************************************************************************************)
+(* HaskWeakTypes: types HaskWeak                                                                                                 *)
+(*********************************************************************************************************************************)
+
+Generalizable All Variables.
+Require Import Preamble.
+Require Import General.
+Require Import Coq.Strings.String.
+Require Import Coq.Lists.List.
+Require Import HaskKinds.
+Require Import HaskCoreLiterals.
+Require Import HaskCoreVars.
+Require Import HaskCoreTypes.
+
+(* TO DO: mark the TyCon used for hetmet as a "type family" so GHC keeps it fully-applied-at-all-times *)
+
+(* a WeakTypeVar merely wraps a CoreVar and includes its Kind *)
+Inductive WeakTypeVar := weakTypeVar : CoreVar -> Kind -> WeakTypeVar.
+
+(*
+ * WeakType is much like CoreType, but:
+ *   1. avoids mutually-inductive definitions
+ *   2. gives special cases for the tycons which have their own typing rules so we can pattern-match on them
+ *   3. separates type functions from type constructors, and uses a normal "AppTy" for applying the latter
+ *)
+Inductive WeakType :=
+| WTyVarTy  : WeakTypeVar                                      -> WeakType
+| WAppTy    : WeakType            ->                  WeakType -> WeakType
+| WTyFunApp : TyCon               ->             list WeakType -> WeakType
+| WTyCon    : TyCon                                            -> WeakType
+| WFunTyCon :                                                     WeakType    (* never use (WTyCon ArrowCon);    always use this! *)
+| WCodeTy   : WeakTypeVar         ->                  WeakType -> WeakType    (* never use the raw tycon *)
+| WCoFunTy  : WeakType            -> WeakType      -> WeakType -> WeakType
+| WForAllTy : WeakTypeVar         ->                  WeakType -> WeakType
+| WClassP   : Class_              ->             list WeakType -> WeakType
+| WIParam   : CoreIPName CoreName ->                  WeakType -> WeakType.
+
+(* EqDecidable instances for WeakType *)
+Instance WeakTypeVarEqDecidable : EqDecidable WeakTypeVar.
+  apply Build_EqDecidable.
+  intros.
+  destruct v1 as [cv1 k1].
+  destruct v2 as [cv2 k2].
+  destruct (eqd_dec cv1 cv2); subst.
+    destruct (eqd_dec k1 k2); subst.
+    left; auto.
+    right; intro; apply n; inversion H; subst; auto.
+    right; intro; apply n; inversion H; subst; auto.
+    Defined.
+
+(* TO DO: write a proper EqDecidable instance for WeakType and then move the rest of this into HaskWeakToCore *)
+Variable ModalBoxTyCon   : TyCon.        Extract Inlined Constant ModalBoxTyCon => "TysWiredIn.hetMetCodeTypeTyCon".
+Variable ArrowTyCon      : TyCon.        Extract Constant ArrowTyCon    => "Type.funTyCon".
+
+(* if this is a (WAppTy (WAppTy ... (WTyCon tc) .. ) .. ), return (tc,[...]) *)
+Fixpoint isTyConApp (wt:WeakType)(acc:list WeakType) : ??(TyCon * list WeakType) :=
+  match wt with
+    | WTyCon tc    => Some (tc,acc)
+    | WAppTy t1 t2 => isTyConApp t1 (t2::acc)
+    | _            => None
+  end.
+
+(* messy first-order NON-CAPTURE-AVOIDING substitution on WeakType's *)
+Fixpoint replaceWeakTypeVar (te:WeakType)(tv:WeakTypeVar)(tsubst:WeakType) : WeakType :=
+  match te with
+    | WTyVarTy  tv'            => if eqd_dec tv tv' then tsubst else te
+    | WAppTy  t1 t2            => WAppTy (replaceWeakTypeVar t1 tv tsubst) (replaceWeakTypeVar t2 tv tsubst)
+    | WForAllTy  tv' t         => if eqd_dec tv tv' then te else WForAllTy tv' (replaceWeakTypeVar t tv tsubst)
+    | WCoFunTy t1 t2 t         => WCoFunTy (replaceWeakTypeVar t1 tv tsubst)
+                                      (replaceWeakTypeVar t2 tv tsubst) (replaceWeakTypeVar t tv tsubst)
+    | WIParam ip ty  => WIParam ip (replaceWeakTypeVar ty tv tsubst)
+    | WClassP  c lt => WClassP c ((fix replaceCoreDistinctList (lt:list WeakType) :=
+      match lt with
+        | nil => nil
+        | h::t => (replaceWeakTypeVar h tv tsubst)::(replaceCoreDistinctList t)
+      end) lt)
+    | WTyFunApp tc lt => WTyFunApp tc ((fix replaceCoreDistinctList (lt:list WeakType) :=
+      match lt with
+        | nil => nil
+        | h::t => (replaceWeakTypeVar h tv tsubst)::(replaceCoreDistinctList t)
+      end) lt)
+    | WTyCon tc                => WTyCon tc
+    | WFunTyCon                => WFunTyCon
+    | WModalBoxTyCon           => WModalBoxTyCon
+  end.
+
+(* we try to normalize the representation of a type as much as possible before feeding it back to GHCs type-comparison function *)
+Definition normalizeWeakType (wt:WeakType) : WeakType := wt.
+
+Fixpoint weakTypeToCoreType' (wt:WeakType) : CoreType :=
+  match wt with
+    | WTyVarTy  (weakTypeVar v _)     => TyVarTy v
+    | WAppTy  t1 t2                   => match (weakTypeToCoreType' t1) with
+                                           | TyConApp tc tys => TyConApp tc (app tys ((weakTypeToCoreType' t2)::nil))
+                                           | t1'             => AppTy t1' (weakTypeToCoreType' t2)
+                                         end
+    | WTyCon    tc                    => TyConApp tc nil
+    | WTyFunApp tc lt                 => TyConApp tc (map weakTypeToCoreType' lt)
+    | WClassP c lt                    => PredTy (ClassP c (map weakTypeToCoreType' lt))
+    | WIParam n ty                    => PredTy (IParam n (weakTypeToCoreType' ty))
+    | WForAllTy (weakTypeVar wtv _) t => ForAllTy wtv (weakTypeToCoreType' t)
+    | WFunTyCon                       => TyConApp ArrowTyCon nil
+    | WCodeTy  (weakTypeVar ec _) t   => TyConApp ModalBoxTyCon ((TyVarTy ec)::(weakTypeToCoreType' t)::nil)
+    | WCoFunTy t1 t2 t3               => FunTy (PredTy (EqPred (weakTypeToCoreType' t1) (weakTypeToCoreType' t2)))
+                                            (weakTypeToCoreType' t3)
+  end.
+
+Definition weakTypeToCoreType (wt:WeakType) :=
+  weakTypeToCoreType' (normalizeWeakType wt).
+
+Definition compare_weakTypes (w1 w2:WeakType) :=
+  if coretype_eq_dec (weakTypeToCoreType w1) (weakTypeToCoreType w2)
+    then true
+    else false.
+
+(* Coq's "decide equality" can't cope here; we have to cheat for now *)
+Axiom compare_weakTypes_axiom : forall w1 w2, if compare_weakTypes w1 w2 then w1=w2 else not (w1=w2).
+
+Instance EqDecidableWeakType : EqDecidable WeakType.
+  apply Build_EqDecidable.
+  intros.
+  set (compare_weakTypes_axiom v1 v2) as x.
+  set (compare_weakTypes v1 v2) as y.
+  assert (y=compare_weakTypes v1 v2). reflexivity.
+  destruct y; rewrite <- H in x.
+  left; auto.
+  right; auto.
+  Defined.
+
+Definition weakTypeToString : WeakType -> string :=
+  coreTypeToString ○ weakTypeToCoreType.
+
